Typing examples

theories/abs_examples.v
@@ -1,5 +1,5 @@
 From ABS Require Import abs_defs.
-From stdpp Require Import prelude.
+From stdpp Require Import prelude base.
 
 (** * ABS Examples *)
 
@@ -12,11 +12,27 @@ Definition func_const_5 : F :=
 Definition e_call_const_5 : e :=
   e_fn_call "const_5"%string [].
 
+Definition Ctx : G :=
+  Map.add ("const_5"%string) (ctxv_sig (sig_sig [] T_int)) (Map.empty ctxv).
+
 Lemma e_const_5_T_int :
- typ_e (Map.empty ctxv) e_const_5 T_int.
+ typ_e Ctx e_const_5 T_int.
 Proof. by apply typ_int. Qed.
 
-Lemma e_call_const_5_T_int :
- typ_e (Map.empty ctxv) e_call_const_5 T_int.
+Lemma e_call_const_typ_F :
+ typ_F Ctx func_const_5.
 Proof.
-Admitted.
+  apply typ_func_decl.
+  - easy.
+  - apply e_const_5_T_int.
+Qed.
+
+Lemma e_call_const_5_T_int :
+ typ_e Ctx e_call_const_5 T_int.
+Proof.
+  unfold e_call_const_5.
+  replace [] with (map (fun (pat_:(e*T)) => match pat_ with (e_,T_) => e_ end ) [])
+    by auto.
+  apply typ_func_expr;
+    easy.
+Qed.
